Instances/Examples/VexMovMemRdiRaxFixture.lean
@@ -13,23 +13,31 @@ def block : Amd64Block :=
   mkAmd64Block [
       .wrTmp 0 (.get .rdi),
       .wrTmp 1 (.get .rax),
-      .store64 (.tmp 0) (.tmp 1)
+      .store .w64 (.tmp 0) (.tmp 1)
     ] 0x400003
 
 def input : Amd64ConcreteState :=
-  mkAmd64State
+  mkAmd64StateCC
     0x1122334455667788
     0x0
     0x20
     0x400000
+    0x0
+    0x0
+    0x0
+    0x0
     (ByteMem.write64le ByteMem.empty 0x20 0xdeadbeefcafebabe)
 
 def expected : Amd64ConcreteState :=
-  mkAmd64State
+  mkAmd64StateCC
     0x1122334455667788
     0x0
     0x20
     0x400003
+    0x0
+    0x0
+    0x0
+    0x0
     (ByteMem.write64le ByteMem.empty 0x20 0x1122334455667788)
 
 end Instances.Examples.VexMovMemRdiRaxFixture
