Instances/Examples/VexMovRaxMemRdiFixture.lean
@@ -12,24 +12,32 @@ def bytes : List UInt8 := [0x48, 0x8b, 0x07]
 def block : Amd64Block :=
   mkAmd64Block [
       .wrTmp 0 (.get .rdi),
-      .wrTmp 1 (.load64 (.tmp 0)),
+      .wrTmp 1 (.load .w64 (.tmp 0)),
       .put .rax (.tmp 1)
     ] 0x400003
 
 def input : Amd64ConcreteState :=
-  mkAmd64State
+  mkAmd64StateCC
     0x0
     0x0
     0x20
     0x400000
+    0x0
+    0x0
+    0x0
+    0x0
     (ByteMem.write64le ByteMem.empty 0x20 0x1122334455667788)
 
 def expected : Amd64ConcreteState :=
-  mkAmd64State
+  mkAmd64StateCC
     0x1122334455667788
     0x0
     0x20
     0x400003
+    0x0
+    0x0
+    0x0
+    0x0
     (ByteMem.write64le ByteMem.empty 0x20 0x1122334455667788)
 
 end Instances.Examples.VexMovRaxMemRdiFixture
